theories/iris_system/syn_invariants.v
@@ -1,85 +1,85 @@
 From stdpp Require Import coPset gmap namespaces.
 From iris Require Import bi.big_op.
-Require Export Coqlib own SRF sProp invariants.
+Require Export Coqlib own SAT sProp invariants.
 
 Local Notation level := nat.
 
 (* Syntactic invariants *)
-Variant inv_shape : Type :=
+Variant inv_ops : Type :=
 | _ownI (u : univ_id) (i : positive)
 | _ownI_auth (u : univ_id) (keys : gmap positive unit)
 | _wsat_auth (u : univ_id).
 
-Local Definition inv_degree (s : inv_shape) (sProp : Type) : Type :=
-  match s with
+Local Definition inv_arity (op : inv_ops) (sProp : Type) : Type :=
+  match op with
   | _ownI u i => fin 1
   | _ownI_auth u keys => positive
   | _wsat_auth u => fin 0
   end.
 
-Global Instance inv_syntax : PF.t := {
-  shp := inv_shape;
-  deg := inv_degree;
+Global Instance inv_syntax : SAT.t := {
+  ops := inv_ops;
+  arity := inv_arity;
 }.
 
 (* Invariant interpretations *)
-Local Definition inv_interp_aux `{!invG α Σ Γ, !subG Γ Σ} n (s : inv_shape) :
-    (inv_degree s (SRFSyn.t_prev n) → SRFSyn.t n) → (inv_degree s (SRFSyn.t_prev n) → iProp Σ)
+Local Definition inv_interp_aux `{!invG α Σ Γ, !subG Γ Σ} n (op : inv_ops) :
+    (inv_arity op (GTerm.t_prev n) → GTerm.t n) → (inv_arity op (GTerm.t_prev n) → iProp Σ)
     → iProp Σ :=
-  match s with
+  match op with
   | _ownI u i => λ syn _, ownI u n i (syn 0%fin)
   | _ownI_auth u keys => λ syn _, ownI_auth u n (map_imap (λ k v, Some (syn k)) keys)
   | _wsat_auth u => λ _ _, wsat_auth u n
   end.
 
 Global Instance inv_interp `{!invG α Σ Γ, !subG Γ Σ} :
-    @SRFIntpM.t (@domain Σ) α _ :=
+    @SATIntp.t (@domain Σ) α _ :=
   inv_interp_aux.
 
-Class syn_invG (Σ : GRA) (Γ : HRA) (α : SRFCons.t) (β : SRFIntp.t) (τ : TypG.t)
+Class syn_invG (Σ : GRA) (Γ : HRA) (α : GAT.t) (β : GATIntp.t) (τ : TypG.t)
     `{!invG α Σ Γ, !subG Γ Σ} := {
-  #[global] syn_invG_inG :: SRFIntp.inG inv_syntax α inv_interp β;
+  #[global] syn_invG_inG :: GATIntp.inG inv_syntax α inv_interp β;
 }.
 
 Section syn_inv.
-  Context `{!invG α Σ Γ, !subG Γ Σ, !CtxST.t τ, !SL.G Σ Γ α β τ, !syn_invG Σ Γ α β τ}.
+  Context `{!invG α Σ Γ, !subG Γ Σ, !GST.t τ, !SL.G Σ Γ α β τ, !syn_invG Σ Γ α β τ}.
   Local Existing Instances invG_Σ invG_Γ invG_I invG_E invG_D.
 
-  Local Definition syn_ownI u n i (p : SRFSyn.t n) : SRFSyn.t n :=
+  Local Definition syn_ownI u n i (p : GTerm.t n) : GTerm.t n :=
     ⟨ _ownI u i, λ _, p ⟩.
-  Local Definition syn_ownI_auth u n (I : gmap positive (SRFSyn.t n)) : SRFSyn.t n :=
-    ⟨ _ownI_auth u (gset_to_gmap tt (dom I)), λ i, or_else (I !! i) emp%SRF⟩.
-  Local Definition syn_wsat_auth u n : SRFSyn.t n :=
+  Local Definition syn_ownI_auth u n (I : gmap positive (GTerm.t n)) : GTerm.t n :=
+    ⟨ _ownI_auth u (gset_to_gmap tt (dom I)), λ i, or_else (I !! i) emp%SAT⟩.
+  Local Definition syn_wsat_auth u n : GTerm.t n :=
     ⟨ _wsat_auth u, λ e, match e with end ⟩.
 
-  Local Definition syn_ownE (u : univ_id) n (E : coPset) : SRFSyn.t n :=
+  Local Definition syn_ownE (u : univ_id) n (E : coPset) : GTerm.t n :=
     <own> base_γ (ownER u E).
-  Local Definition syn_ownD (u : univ_id) n (D : gset positive) : SRFSyn.t n :=
+  Local Definition syn_ownD (u : univ_id) n (D : gset positive) : GTerm.t n :=
     <own> base_γ (ownDR u D).
-  Local Definition syn_ownD_auth (u : univ_id) n : SRFSyn.t n :=
-    (∃ D : τ{⇣gset positive}, <own> base_γ (ownD_authR u D))%SRF.
+  Local Definition syn_ownD_auth (u : univ_id) n : GTerm.t n :=
+    (∃ D : τ{⇣gset positive}, <own> base_γ (ownD_authR u D))%SAT.
 
-  Local Definition syn_inv_satall u n (I : gmap positive (SRFSyn.t n)) : SRFSyn.t n :=
-    ([∗ n map] i ↦ p ∈ I, (p ∗ syn_ownD u n {[i]}) ∨ syn_ownE u n {[i]})%SRF.
-  Local Definition syn_wsat u n : SRFSyn.t (S n) :=
-    (∃ I : τ{ST.gmapT Φ}, (⤉ syn_ownI_auth u n I) ∗ (⤉ syn_inv_satall u n I))%SRF.
+  Local Definition syn_inv_satall u n (I : gmap positive (GTerm.t n)) : GTerm.t n :=
+    ([∗ n map] i ↦ p ∈ I, (p ∗ syn_ownD u n {[i]}) ∨ syn_ownE u n {[i]})%SAT.
+  Local Definition syn_wsat u n : GTerm.t (S n) :=
+    (∃ I : τ{ST.gmapT Φ}, (⤉ syn_ownI_auth u n I) ∗ (⤉ syn_inv_satall u n I))%SAT.
 
-  Local Fixpoint syn_wsatl u n : SRFSyn.t n :=
+  Local Fixpoint syn_wsatl u n : GTerm.t n :=
     match n with
-    | O => emp%SRF
+    | O => emp%SAT
     | S n' => syn_wsat u n' ∗ ⤉ syn_wsatl u n'
     end.
-  Local Definition syn_wsats u n (E : coPset) : SRFSyn.t n :=
+  Local Definition syn_wsats u n (E : coPset) : GTerm.t n :=
     syn_wsat_auth u n ∗ syn_ownE u n E ∗ syn_ownD_auth u n ∗ syn_wsatl u n.
 
   (* Interface for the user *)
   Local Definition syn_inv_def (u : univ_id) (n : level) (N : namespace) p :=
-    (∃ i : τ{⇣positive}, ⌜i ∈ (↑N : coPset)⌝ ∧ syn_ownI u n i p)%SRF.
+    (∃ i : τ{⇣positive}, ⌜i ∈ (↑N : coPset)⌝ ∧ syn_ownI u n i p)%SAT.
   Local Definition syn_inv_aux : seal (@syn_inv_def). Proof. by eexists. Qed.
   Definition syn_inv := syn_inv_aux.(unseal).
   Local Definition syn_inv_eq : @syn_inv = @syn_inv_def := syn_inv_aux.(seal_eq).
 
-  Local Definition syn_fupd_def u b (E1 E2 : coPset) (P : SRFSyn.t b) : SRFSyn.t b :=
+  Local Definition syn_fupd_def u b (E1 E2 : coPset) (P : GTerm.t b) : GTerm.t b :=
     syn_wsatl u b ∗ syn_ownE u b E1 ∗ syn_ownD_auth u b
     ==∗ (syn_wsatl u b ∗ syn_ownE u b E2 ∗ syn_ownD_auth u b ∗ P).
   Local Definition syn_fupd_aux : seal (@syn_fupd_def). Proof. by eexists. Qed.
@@ -87,9 +87,9 @@ Section syn_inv.
   Local Definition syn_fupd_eq : @syn_fupd = @syn_fupd_def := syn_fupd_aux.(seal_eq).
 End syn_inv.
 
-Class sinvG (Σ : GRA) (Γ : HRA) (α : SRFCons.t) (β : SRFIntp.t) (τ : TypG.t)
+Class sinvG (Σ : GRA) (Γ : HRA) (α : GAT.t) (β : GATIntp.t) (τ : TypG.t)
     `{!invG α Σ Γ, !subG Γ Σ} := sinvG_mk {
-  #[global] sinv_typG :: CtxST.t τ;
+  #[global] sinv_typG :: GST.t τ;
   #[global] sinv_SLG :: SL.G Σ Γ α β τ;
   #[global] sinv_syn_invG :: syn_invG Σ Γ α β τ;
 }.
@@ -99,7 +99,7 @@ Section reduction.
   Lemma ownI_auth_red u n I :
     ⟦syn_ownI_auth u n I⟧ = ownI_auth u n I.
   Proof.
-    SRF_red; ss.
+    SAT_red; ss.
     f_equal. apply map_eq; intros i.
     destruct (decide (i ∈ dom I)).
     { rewrite map_lookup_imap lookup_gset_to_gmap //=. case_guard; ss. apply elem_of_dom in e; ss.
@@ -112,14 +112,14 @@ Section reduction.
 
   Lemma wsat_red u n : ⟦syn_wsat u n⟧ ≡ wsat u n.
   Proof.
-    rewrite /syn_wsat /wsat; SRF_red; SL_red.
+    rewrite /syn_wsat /wsat; SAT_red; SL_red.
     iSplit; iIntros "[%I H]"; SL_red.
-    { rewrite @SRFRed.lift ownI_auth_red. SRF_red. rewrite /syn_inv_satall; SL_red.
+    { rewrite @SATRed.lift ownI_auth_red. SAT_red. rewrite /syn_inv_satall; SL_red.
       iExists I; iDestruct "H" as "[$ H]".
       rewrite /inv_satall. iApply (big_sepM_mono with "H"); ss.
       rewrite /ownD /ownE. intros k x IN; SL_red; ss.
     }
-    { iExists I; SL_red; rewrite !@SRFRed.lift ownI_auth_red /syn_inv_satall; SL_red.
+    { iExists I; SL_red; rewrite !@SATRed.lift ownI_auth_red /syn_inv_satall; SL_red.
       iDestruct "H" as "[$ H]".
       rewrite /inv_satall. iApply (big_sepM_mono with "H"); ss.
       rewrite /ownD /ownE. intros k x IN; SL_red; ss.
@@ -129,17 +129,17 @@ Section reduction.
   Lemma wsatl_red u n : ⟦syn_wsatl u n⟧ ≡ wsatl u n.
   Proof.
     induction n.
-    { SRF_red; SL_red; ss. }
-    { simpl syn_wsatl. SRF_red; ss. rewrite /wsatl seq_S big_sepL_app //=.
-      rewrite wsat_red; SRF_red; rewrite IHn; iSplit; iIntros "[$ H]"; iFrame.
+    { SAT_red; SL_red; ss. }
+    { simpl syn_wsatl. SAT_red; ss. rewrite /wsatl seq_S big_sepL_app //=.
+      rewrite wsat_red; SAT_red; rewrite IHn; iSplit; iIntros "[$ H]"; iFrame.
       iDestruct "H" as "[??]"; iFrame.
     }
   Qed.
   
   Lemma wsats_red u n E : ⟦syn_wsats u n E⟧ ≡ wsats u n E.
   Proof.
-    rewrite /syn_wsats /syn_ownE /syn_ownD_auth. SRF_red. SL_red.
-    rewrite wsatl_red; SRF_red; ss; rewrite /wsats /ownD_auth.
+    rewrite /syn_wsats /syn_ownE /syn_ownD_auth. SAT_red. SL_red.
+    rewrite wsatl_red; SAT_red; ss; rewrite /wsats /ownD_auth.
     iSplit; iIntros "($ & $ & [%x H] & $)"; iExists x; SL_red; iFrame.
   Qed.
 
@@ -147,13 +147,13 @@ Section reduction.
   Proof.
     rewrite syn_inv_eq /syn_inv_def. SL_red.
     rewrite /inv invariants.inv_aux.(seal_eq) /invariants.inv_def.
-    iSplit; iIntros "[%x H]"; iExists x; SL_red; SRF_red; ss.
+    iSplit; iIntros "[%x H]"; iExists x; SL_red; SAT_red; ss.
   Qed.
 
   Lemma fupd_red u n E1 E2 P : ⟦syn_fupd u n E1 E2 P⟧ ≡ uPred_fupd u n E1 E2 ⟦P⟧.
   Proof.
     rewrite syn_fupd_eq /uPred_fupd invariants.uPred_fupd_aux.(seal_eq) /invariants.uPred_fupd_def.
-    rewrite /syn_fupd_def SLRed.wand SLRed.upd. repeat SRF_red.
+    rewrite /syn_fupd_def SLRed.wand SLRed.upd. repeat SAT_red.
     rewrite wsatl_red /wsatl /syn_ownE /syn_ownD_auth; SL_red.
     iSplit; iIntros "I [W [E [%x D]]]"; iMod ("I" with "[W E D]") as "[$ [$ [[%x' I] $]]]"; SL_red; iFrame.
     all: ss; iExists _; SL_red; ss.
@@ -167,17 +167,17 @@ Ltac inv_red :=
 Module inv_instances.
   #[export] Instance τ : TypG.t := λ _, ST.t.
 
-  #[export] Instance typG : CtxST.t τ.
+  #[export] Instance typG : GST.t τ.
   Proof. econs. econs. instantiate (1:=0); ss. Qed.
 
-  #[export] Instance α {Γ : HRA} : SRFCons.t :=
+  #[export] Instance α {Γ : HRA} : GAT.t :=
     λ n,
       match n with
       | 0 => SL.syntax
       | _ => inv_syntax
       end.
 
-  #[export] Instance β {Σ : GRA} {Γ : HRA} `{!subG Γ Σ, !invG α Σ Γ} : SRFIntp.t :=
+  #[export] Instance β {Σ : GRA} {Γ : HRA} `{!subG Γ Σ, !invG α Σ Γ} : GATIntp.t :=
     λ n,
       match n with
       | 0 => SL.interp
@@ -185,11 +185,11 @@ Module inv_instances.
       end.
 
   #[export] Instance intpG {Σ : GRA} {Γ : HRA} `{!subG Γ Σ, !invG α Σ Γ} :
-    SRFIntp.inG (@SL.syntax τ Γ) α (@SL.interp τ α Γ Σ _) β.
+    GATIntp.inG (@SL.syntax τ Γ) α (@SL.interp τ α Γ Σ _) β.
   Proof. econs; instantiate (1:=0); ss. Qed.
 
   #[export] Instance invintpG {Σ : GRA} {Γ : HRA} `{!subG Γ Σ, !invG α Σ Γ} :
-    SRFIntp.inG inv_syntax α inv_interp β.
+    GATIntp.inG inv_syntax α inv_interp β.
   Proof. econs; instantiate (1:=1); ss. Qed.
 
   #[export] Instance sinvg {Σ : GRA} {Γ : HRA} `{!subG Γ Σ, !invG α Σ Γ} : sinvG Σ Γ α β τ.
