theories/common/Common.v
@@ -2,7 +2,7 @@ Require Export Program Permutation Orders String HexString ZArith.
 
 Require Export Axioms Any AList Red IRed SubPerm.
 Require Export sflib Coqlib ITreelib.
-Require Export own SRF invariants sProp syn_invariants.
+Require Export SAT own invariants sProp syn_invariants.
 Require Export Events Behavior.
 
 (* TODO: Move *)
