theories/lib/SAT.v
@@ -1,0 +1,208 @@
+Require Import sflib Basics Program.
+
+Definition level := nat.
+
+(****
+
+ Library for Polynomial Functors
+
+ ****)
+
+(* Stratified Algebraic Theory *)
+
+Module SAT.
+
+  Class t : Type := {
+    ops : Type;
+    arity : ops -> forall (term_prev: Type), Type;
+  }.
+
+End SAT.
+
+(* Global Algebraic Theory *)
+Module GAT.
+
+  Class t : Type := __GATOM : nat -> SAT.t.
+
+  Class inG (F : SAT.t) (GF : t) : Type := {
+    inG_id : nat;
+    inG_prf : F = GF inG_id;
+  }.
+
+End GAT.
+
+(****
+
+ Library for SAT
+
+ ****)
+
+(* Term *)
+Module GTerm. Section GTerm.
+  Context `{α: GAT.t}.
+
+  Inductive term {term_prev: Type} : Type :=
+  | _lift (p: term_prev) : term
+  | _cur i (op: (α i).(SAT.ops)) (args: (α i).(SAT.arity) op term_prev -> term)
+  .
+
+  Fixpoint _t (n : level) : Type :=
+    match n with
+    | O => Empty_set
+    | S m => term (term_prev:=_t m) 
+    end.
+
+  Definition t_prev (n : level) : Type := _t n.
+
+  Definition t (n : level) : Type := t_prev (S n).
+
+  Definition lift {n} (p : t n) : t (S n) := _lift p.
+
+  Fixpoint liftn k {n} (p : t n) : t (k+n) :=
+    match k return t (k+n) with
+    | 0 => p
+    | S k' => lift (liftn k' p)
+    end.
+End GTerm. End GTerm.
+
+(* Semantic Domain *)
+Module SemDom.
+
+  Class t : Type := {
+      dom: Type;
+    }.
+
+End SemDom.
+
+(* Interpretation for the constructors in a group *)
+Module SATIntp.
+
+  Section SEM.
+
+  Context `{Δ: SemDom.t}.
+  Context `{α: GAT.t}.
+  Context `{A: SAT.t}.
+
+  Class t : Type := 
+    sem:
+      forall n (op: A.(SAT.ops))
+             (args: A.(SAT.arity) op (@GTerm.t_prev α n) -> GTerm.t n)
+             (Args: A.(SAT.arity) op (@GTerm.t_prev α n) -> SemDom.dom),
+        SemDom.dom
+  .
+
+  End SEM.
+
+End SATIntp.
+
+(* Interpretation for the constructors in all groups *)
+Module GATIntp.
+
+  Section GSEM.
+
+  Context `{Δ : SemDom.t}.
+
+  Class t `{α: GAT.t}: Type :=
+    gsem : forall i, @SATIntp.t Δ α (α i).
+
+  Class inG (A: SAT.t) (α: GAT.t) (B: @SATIntp.t Δ α A) (β: t) :=
+    {
+      inG_id: nat;
+      inG_prf: existT _ A B = existT _ (α inG_id) (β inG_id);
+    }.
+  
+  End GSEM.
+
+End GATIntp.
+
+(* Semantics for the syntax *)
+Module GTermSem.
+
+  Section SEM.
+
+  Context `{Δ: SemDom.t}.
+  Context `{α: GAT.t}.
+  Context `{β: @GATIntp.t Δ α}.
+
+  Fixpoint _t n : GTerm.t_prev n -> SemDom.dom :=
+    match n with
+    | O => fun x => match x with end
+    | S m =>
+      fix _t_aux (syn : GTerm.t_prev (S m)) : SemDom.dom :=
+        match syn with
+        | GTerm._lift p => _t m p
+        | GTerm._cur i op args => β i m op args (compose _t_aux args)
+        end
+    end.
+
+  Definition t_prev n : GTerm.t_prev n -> SemDom.dom := _t n.
+  
+  Definition t n : GTerm.t n -> SemDom.dom := t_prev (S n).
+
+  Program Definition cur
+    `{A: SAT.t} `{B: @SATIntp.t Δ α A} `{IN: @GATIntp.inG Δ A α B β} {n}
+    (op: A.(SAT.ops)) (args: A.(SAT.arity) op (GTerm.t_prev n) -> GTerm.t n) : GTerm.t n.
+    destruct IN. inversion inG_prf. subst.
+    exact (GTerm._cur inG_id op args).
+  Defined.
+  
+  End SEM.
+  
+End GTermSem.
+
+Module SATRed.
+  
+  Section RED.
+
+  Context `{Δ: SemDom.t}.
+  Context `{α: GAT.t}.
+  Context `{β: @GATIntp.t Δ α}.
+
+  Lemma cur `{A: SAT.t} `{B: @SATIntp.t Δ α A} `{IN: @GATIntp.inG Δ A α B β} n op args:
+    GTermSem.t n (GTermSem.cur op args) = B n op args (compose (GTermSem.t n) args).
+  Proof.
+    destruct IN eqn : EQ. subst. dependent destruction inG_prf. reflexivity.
+  Qed.
+
+  Lemma lift_0 t d:
+    GTermSem.t_prev 1 (GTerm._lift t) = d.
+  Proof. destruct t. Qed.
+
+  Lemma lift n (t : GTerm.t n) :
+    GTermSem.t (S n) (GTerm.lift t) = GTermSem.t n t.
+  Proof. reflexivity. Qed.
+
+  End RED.
+
+End SATRed.
+
+Global Opaque GTermSem.cur.
+Global Opaque GTermSem.t.
+
+(** Notations *)
+
+Declare Scope SAT_scope.
+Delimit Scope SAT_scope with SAT.
+Bind Scope SAT_scope with GTerm.t.
+
+Local Open Scope SAT_scope.
+
+Notation "'⟦' F ',' n '⟧'" := (GTermSem.t n F).
+Notation "'⟦' F '⟧'" := (GTermSem.t _ F).
+Notation "'⟨' op ',' args '⟩'" := (GTermSem.cur op args) : SAT_scope.
+Notation "⤉ P" := (GTerm.lift P) (at level 20) : SAT_scope.
+
+(* Simple reduction tactics. *)
+
+Global Opaque GTerm.t_prev.
+Global Opaque GTerm.t.
+
+(* TODO : improve these tactics *)
+From stdpp Require Import ssreflect.
+Ltac SAT_red :=
+  (hrepeat do 1
+    tryany (do 1 rewrite !@SATRed.cur)
+    tryany (do 1 rewrite !@SATRed.lift)
+           (try (change (GTerm.t_prev (S ?n)) with (); fail 1);
+            change (GTerm.t_prev (S ?n)) with (GTerm.t n)));
+  simpl.
